%\chapter\veeesults}

%\input{discussion}

\section*{1}
\begin{enumerate}
    \item
        \begin{table}[h]
            \centering
            \begin{tabular}{l|l|l|l|l|l}
                \hline
                1,3 & 2,2 & 3,1 & KB & $\alpha_2$ & $\alpha_3$ \\\hline
                ~  & ~  & ~  & ~ & T & ~ \\
                P  & ~  & ~  & ~ & T & ~ \\
                W  & ~  & ~  & ~ & T & T \\
                PW & ~  & ~  & ~ & T & T \\
                ~  & P  & ~  & ~ & ~ & ~ \\
                P  & P  & ~  & ~ & ~ & ~ \\
                W  & P  & ~  & ~ & ~ & T \\
                PW & P  & ~  & ~ & ~ & T \\
                ~  & W  & ~  & ~ & T & ~ \\
                P  & W  & ~  & ~ & T & ~ \\
                ~  & PW & ~  & ~ & ~ & ~ \\
                P  & PW & ~  & ~ & ~ & ~ \\
                ~  & ~  & P  & ~ & T & ~ \\
                P  & ~  & P  & ~ & T & ~ \\
                W  & ~  & P  & T & T & T \\
                PW & ~  & P  & ~ & T & T \\
                ~  & P  & P  & ~ & ~ & ~ \\
                P  & P  & P  & ~ & ~ & ~ \\
                W  & P  & P  & ~ & ~ & T \\
                PW & P  & P  & ~ & ~ & T \\
                ~  & W  & P  & ~ & T & ~ \\
                P  & W  & P  & ~ & T & ~ \\
                ~  & PW & P  & ~ & ~ & ~ \\
                P  & PW & P  & ~ & ~ & ~ \\
                ~  & ~  & W  & ~ & T & ~ \\
                P  & ~  & W  & ~ & T & ~ \\
                ~  & P  & W  & ~ & ~ & ~ \\
                P  & P  & W  & ~ & ~ & ~ \\
                ~  & ~  & PW & ~ & T & ~ \\
                P  & ~  & PW & ~ & T & ~ \\
                ~  & P  & PW & ~ & ~ & ~ \\
                P  & P  & PW & ~ & ~ & ~ \\
            \end{tabular}
            \caption {Wumpus}
        \end{table}
        We can see that $\text{KB} \models \alpha_2$ and $\text{KB} \models \alpha_3$ since the single row with $\text{KB} = \text{True}$ has both $\alpha_2$ and $\alpha_3$ True.

    \item

        \begin{enumerate}[a.]
            \item True, False is never true, ergo this statement doesn't violate the definition of entailment.
            \item False. Inverse of above, False is never true, and the statement will therefore always violate the definition.
            \item True. $M(\text{LHS}) \subseteq M(\text{RHS})$
            \item False. With both $A$ and $B$ True, the LHS will be true, but the RHS will be false. Thus $M(\text{LHS}) \not\subseteq M(\text{RHS})$.
            \item True. $M(\text{LHS}) = M(\text{RHS})$ for this statement.
            \item True. The only case that would make the right hand side False is $A = B = \text{True}, C = False$ for which the LHS is also false.
        \end{enumerate}
    \item
        \begin{enumerate}[a.]
            \item $\{T, F\}, \{TF, FT, TT\}, \{T, F\}$. $2*3*2 = 12$
            \item Only false if all propositions are True, therefore $2^4 - 1 = 15$ models.
            \item $0$. $A = T, B = F$ means that $A \implies B$ can never be true.
        \end{enumerate}

    \item
        \begin{enumerate}[a.]
            \item Valid. $\text{Smoke} \implies \text{Smoke} \equiv \neg \text{Smoke} \vee \text{Smoke}$
            \item Neither. All models except $\text{Smoke} = \text{True}, \text{Fire} = \text{False}$ satisfies the sentence.
            \item Neither. 
                \begin{gather*}
                    (\text{Smoke} \implies \text{Fire}) \implies (\neg \text{Smoke} \implies \neg \text{Fire})
                    \equiv (\neg \text{Smoke} \vee \text{Fire} \implies \neg \text{Fire} \vee \text{Smoke})
                \end{gather*}
                False for $\text{Smoke} = \text{False}, \text{Fire} = \text{True}$
        \end{enumerate}
    \item
        \begin{enumerate}[a.]
            \item $^3/_4 Q$
            \item $^5/_8 Q$
            \item $^3/_4 Q$
        \end{enumerate}
\end{enumerate}

\section*{2}
\subsection*{1}
\begin{enumerate}
    \item $A \wedge B \wedge C$
    \item $A \vee B \vee C$
    \item $\neg A \vee B \vee C$
    \item $(\neg A \vee C) \wedge (B \vee C)$
    \item $\neg A \vee \neg B \vee C \vee D$
    \item $(\neg A \vee C) \wedge (\neg A \vee D) \wedge (\neg B \vee C) \wedge (\neg B) \vee D)$
    \item $(\neg A \vee \neg B \vee C) \wedge (A \vee \neg C) \wedge (B \vee \neg C)$
\end{enumerate}
\subsection*{2}
The items in the KB individually CNF to:
\begin{itemize}
    \item   $(\neg A \vee  \neg C) \wedge  (B \vee  \neg C)$
    \item   $(C \vee  \neg E) \wedge  D$
    \item   $A \wedge D$
\end{itemize}

Since these statements are the KB, we can and them together, and simplify:
\begin{align*}
(\neg A \vee  \neg C) \wedge  (B \vee  \neg C) \wedge (C \vee  \neg E) \wedge  D \wedge A \wedge D
\\
(\neg A \vee  \neg C) \wedge  (B \vee  \neg C) \wedge (C \vee  \neg E) \wedge  D \wedge A
\\
\neg C \wedge  (B \vee  \neg C) \wedge (C \vee  \neg E) \wedge  D \wedge A
\\
\neg C \wedge  B \wedge \neg E \wedge  D \wedge A
\end{align*}
And at this point we can see that for the KB to hold true, we must have $\neg E$.


\section*{3}
\subsection*{1}
\begin{enumerate}[a.]
    \item $\text{Occupation}(\text{Emily}, \text{Lawyer}) \vee \text{Occupation}(\text{Emily}, \text{Surgeon})$
    \item $\text{Occupation}(\text{Joe}, \text{Actor}) \wedge \exists o \{\text{Occupation}(\text{Joe}, o)\}$
    \item $\forall x \{\text{Occupation}(x, Doctor) \wedge \text{Occupation}(x, Surgeon)\}$
\end{enumerate}

\subsection*{2}
\begin{enumerate}[a.]
    \item $\forall x \{ \text{Even}(x) \Leftrightarrow \exists y \{ x = y + y\}\}$
    \item $\forall x \{ \text{Prime}(x) \Leftrightarrow \forall yz \{ x = y \times z \implies z = 1 \vee y = 1\}\}$
    \item $\forall x \{ \text{Even}(x) \Leftrightarrow \exists yz \{ x = y + z \wedge (\text{Prime}(y) \wedge \text{Prime}(z))\}\}$
\end{enumerate}

\subsection*{3}
\begin{gather*}
    \forall k \{ \text{Key}(k) \implies \exists t_0 \{\text{Before}(\text{Now}, t_0) \wedge \forall t \{ \text{Before}(t_0, t) \implies \text{Lost}(k, t)\} \} \\
    \forall xy \{ \text{Sock}(x) \wedge \text{Sock}(y) \wedge \text{Pair}(x, y) \implies \\
    \exists t_1 \{ \text{Before}(Now, t_1) \wedge \forall t \{ \text{Before}(t_1, t) \wedge \text{Lost}(x, t)\} \} \vee \\
    \exists t_2 \{ \text{Before}(Now, t_2) \wedge \forall t \{ \text{Before}(t_2, t) \wedge \text{Lost}(y, t)\} \} \}
\end{gather*}

\subsection*{4}
With the following vocabulary:
\begin{gather*}
    V = \{\text{Person}(x), \text{IsDNAOfPerson}(x, y), \text{IsParentOf}(x, y), \text{IsDerivedFromPersonsDNA}(x, y)\}
\end{gather*}

where $\text{Person}(x)$ is true if $x$ is a person, $\text{IsDNAOfPerson}(x, y)$ is true if $y$ is person $x$'s DNA, $\text{IsParentOf}(x, y)$ is true if $y$ is $x$'s parent and $\text{IsDerivedFromPersonsDNA}(x, y)$ is true if DNA $x$ is derived from person $x$'s DNA.
\begin{gather*}
    \forall xy \{ \text{Person}(x) \wedge \text{IsDNAOfPerson}(y, x) \implies \neg \exists z \{ \text{Person}(z) \wedge \text{IsDNAOfPerson}(y, z) \} \wedge \\
    \forall a \{ \text{Person}(a) \wedge \text{IsParentOf}(x, a) \implies \text{IsDerivedFromPersonsDNA}(y, a) \}\}
\end{gather*}


\section*{4}
\subsection*{1}
\begin{enumerate}[a.]
    \item $\Theta = \{x/\text{Rocky}\}$
    \item $\Theta = \{x/\text{Leo}, y/\text{Rocky}\}$
    \item $\Theta = \{x/\text{Rocky}, y/\text{Leo}\}$
    \item Not possible.
    \item Not Possible.
    \item $\Theta = \{x/\text{Leo}, y/\text{FastestHorse(x)}\}$
    \item $\Theta = \{x/\text{Marvin}, y/\text{Leo}\}$
\end{enumerate}

\subsection*{2}

Only the last sentence needs to be converted to CNF.

\begin{gather*}
    \forall x \{ \text{Green}(x) \leftrightarrow \text{Bikes}(x) \vee \exists y \{ \text{Drives}(x, y) \wedge \text{Hybrid}(y) \} \}
\end{gather*}
